Developing theory of thinning clauses to avoid "latent" loops

common/theories/LoopChecking/Deciders.v
@@ -1452,7 +1452,7 @@ Module CorrectModel.
     rewrite initm in hle. rewrite -/(model_of m) in ext hle. lia.
   Qed.
 
-  Lemma model_max {V cls} {m : t V cls}: forall l k, LevelMap.MapsTo l (Some k) (model_of m) ->
+  Lemma model_max_0 {V cls} {m : t V cls}: forall l k, LevelMap.MapsTo l (Some k) (model_of m) ->
      (Some k ≤ level_value (model_of m) (Level.zero))%opt.
   Proof.
     intros l k hm.
@@ -1534,7 +1534,7 @@ Module CorrectModel.
     have zerom := model_max_spec m _ _ hzero. depelim zerom.
     destruct mmax'. rewrite H0 in H. cbn in *. lia.
     destruct H0 as [l' [k' [hm' eqmax]]].
-    move/model_max: hm'. rewrite (level_value_MapsTo hzero) => hle; depelim hle.
+    move/model_max_0: hm'. rewrite (level_value_MapsTo hzero) => hle; depelim hle.
     have mr := valuation_range hzero. subst k'.
     have hs := valuation_of_model_spec (model_of m) _ _ hzero.
     cbn in hs.
@@ -2354,6 +2354,23 @@ Lemma opt_valuation_of_model_equiv m l :
     exists z. split => //.
   Qed.
 
+  Lemma clause_sem_defined_premises_valid {model cl} :
+    defined_model_of (NES.levels (premise cl)) model ->
+    clause_sem (opt_valuation_of_model model) cl -> clause_sem (Z_valuation_of_model model) cl.
+  Proof.
+    intros def.
+    destruct cl as [prems [concl k]].
+    rewrite /clause_sem. rewrite interp_nes_defined //.
+    unfold interp_expr.
+    destruct (opt_valuation_of_model model concl) eqn:hconcl.
+    * eapply opt_valuation_of_model_inv in hconcl as [k' [hm heq]]. subst z.
+      cbn. rewrite {3}/Z_valuation_of_model /to_Z_val /to_val.
+      have hv := valuation_of_value_pos hm.
+      apply valuation_of_model_spec in hm.
+      rewrite (LevelMap.find_1 hm). rewrite -/(valuation_of_value model k').
+      lia.
+    * now cbn.
+  Qed.
 
   Lemma clause_sem_defined_valid_all {model cl} :
     defined_model_of (clause_levels cl) model ->
@@ -3031,18 +3048,21 @@ Proof.
 Qed.
 
 Definition valid_total_models cls cl :=
-  forall m : Model.model, is_total_model m cls -> defined_model_of (clause_levels cl) m -> valid_clause m cl.
+  forall m : Model.model, is_total_model m cls ->
+  defined_model_of (clause_levels cl) m -> valid_clause m cl.
 
-Lemma valid_total_models_Z_models cls cl : valid_clause_Z cls cl -> valid_total_models cls cl.
+Lemma valid_total_models_Z_models cls cl : valid_clause_Z cls cl <-> valid_total_models cls cl.
 Proof.
-  intros H m istot encl.
-  move: (H (Z_valuation_of_model m)) => /fwd.
-  eapply valuation_of_model_pos.
-  move=> /fwd. destruct istot. move/is_modelP: H1 => H1.
-  move=> cl' /[dup] /H0 en /H1.
-  now eapply valid_clause_model.
-  intros cs.
-  rewrite -def_clause_sem_valid //.
+  split.
+  - intros H m istot encl.
+    move: (H (Z_valuation_of_model m)) => /fwd.
+    eapply valuation_of_model_pos.
+    move=> /fwd. destruct istot. move/is_modelP: H1 => H1.
+    move=> cl' /[dup] /H0 en /H1.
+    now eapply valid_clause_model.
+    intros cs.
+    rewrite -def_clause_sem_valid //.
+  - intros vm v vpos csem. todo "admit".
 Qed.
 
 
@@ -3073,9 +3093,95 @@ Proof.
       apply LevelExprSet.singleton_spec in hadd. red in hadd. congruence.
 Qed.
 
+
+Module CounterExample1.
 (* x ∨ y -> y + 1 *)
 Definition valid_Z_counterexample_cls (x y : Level.t) : clause :=
   ((singleton (x, 0) ∨ singleton (y, 0)), (y, 1))%nes.
+
+(* x -> y + 1 *)
+Definition valid_Z_counterexample_cl (x y : Level.t) : clause :=
+  (singleton (x, 0), (y, 1))%nes.
+
+Example check_clause_invalid_Z_counterexample (x y : Level.t) :
+  x <> y ->
+  let cls := Clauses.singleton (valid_Z_counterexample_cls x y) in
+  let cl := valid_Z_counterexample_cl x y in
+  exists mcheck, check_gen cls cl = Invalid mcheck /\ valid_clause_Z cls cl.
+Proof.
+  move=> hdiff cls cl.
+  set (v := (fun l : Level.t => if eqb l x then 1 else 0)%Z).
+  have vx : v x = 1. now rewrite /v eqb_refl.
+  have vy : v y = 0. rewrite /v. case: eqb_spec => //. subst; congruence.
+  have hcls : clauses_sem v cls.
+  { eapply clauses_sem_singleton. cbn.
+    rewrite interp_nes_union !interp_nes_singleton //=.
+    rewrite vx vy. cbn. lia. }
+  have hcon : consistent cls.
+  { exists v. split => //.
+    intros l. unfold v. case: eqb_spec => //. }
+  destruct check_gen eqn:ec.
+  - move/check_gen_entails_looping: ec.
+    move/consistent_no_loop. contradiction.
+  - exists m. split => //.
+    intros v' vpos csem.
+    unfold cl; cbn.
+    rewrite interp_nes_singleton //=.
+    move: (csem (valid_Z_counterexample_cls x y)) => /fwd. now eapply Clauses.singleton_spec.
+    cbn. rewrite !interp_nes_union !interp_nes_singleton //=. lia.
+  - exfalso. move/check_gen_entails: ec.
+    rewrite entails_completeness.
+    intros ent.
+    set (vopt := (fun l : Level.t => if eqb l x then Some 0 else None)%Z).
+    have voptx : vopt x = Some 0. now rewrite /vopt eqb_refl.
+    have vopty : vopt y = None. rewrite /vopt. case: eqb_spec => //. subst; congruence.
+    specialize (ent (option Z) _ vopt).
+    have hcls' : clauses_sem vopt cls.
+    { eapply clauses_sem_singleton. cbn.
+      rewrite interp_nes_union !interp_nes_singleton //=.
+      rewrite voptx vopty. now cbn. }
+    move: (ent hcls'); cbn.
+    rewrite !interp_nes_singleton //=.
+    now rewrite voptx vopty; cbn.
+Qed.
+
+Example check_clause_checking_invalid_Z_example (x y : Level.t) :
+  x <> y ->
+  let cls := Clauses.singleton (valid_Z_counterexample_cls x y) in
+  let cl := valid_Z_counterexample_cl x y in
+  check_gen cls (checking_clause cl) = Valid.
+Proof.
+  move=> hdiff cls cl.
+  set (v := (fun l : Level.t => if eqb l x then 1 else 0)%Z).
+  have vx : v x = 1. now rewrite /v eqb_refl.
+  have vy : v y = 0. rewrite /v. case: eqb_spec => //. subst; congruence.
+  have hcls : clauses_sem v cls.
+  { eapply clauses_sem_singleton. cbn.
+    rewrite interp_nes_union !interp_nes_singleton //=.
+    rewrite vx vy. cbn. lia. }
+  have hcon : consistent cls.
+  { exists v. split => //.
+    intros l. unfold v. case: eqb_spec => //. }
+  destruct check_gen eqn:ec.
+  - move/check_gen_entails_looping: ec.
+    move/consistent_no_loop. contradiction.
+  - exfalso. move/check_invalid_entails: ec.
+    apply. apply entails_completeness.
+    red. intros.
+    move: (H (valid_Z_counterexample_cls x y)) => /fwd.
+    now apply Clauses.singleton_spec.
+    cbn. rewrite !interp_nes_union !interp_nes_singleton //=.
+    rewrite !add_neutral. intros hle.
+    now rewrite join_comm.
+  - reflexivity.
+Qed.
+
+End CounterExample1.
+
+Module CounterExample2.
+(* x + 1 ∨ y -> y + 1 *)
+Definition valid_Z_counterexample_cls (x y : Level.t) : clause :=
+  ((singleton (x, 1) ∨ singleton (y, 0)), (y, 1))%nes.
 
 (* x -> y *)
 Definition valid_Z_counterexample_cl (x y : Level.t) : clause :=
@@ -3150,14 +3256,507 @@ Proof.
     now apply Clauses.singleton_spec.
     cbn. rewrite !interp_nes_union !interp_nes_singleton //=.
     rewrite !add_neutral. intros hle.
-    apply (le_add (n:=1)).
-    etransitivity; tea.
-    rewrite !add_join !add_distr.
-    have -> : (1 + (0 - 1))%Q = 0 by cbn; lia.
-    rewrite add_neutral join_comm.
-    eapply join_le_pres. reflexivity.
-    red. now rewrite join_sub.
+    eapply (le_add (n := 1)).
+    rewrite !add_join !add_distr add_neutral join_comm.
+    exact hle.
   - reflexivity.
+Qed.
+
+End CounterExample2.
+
+(** To ensure validity in Z, one must remove "latent" loops from the clauses.
+  As we start validity checking from a set of satisfiable clauses, we know
+  that there exists an equivalent set of clauses (for Z valuations) with
+  no latent loop.
+  It is basically computed by the inference algorithm.
+
+  E.g. if we encountered a clause l ∨ x + 1 -> l+1 during inference and found
+  a total model m of this clause, then necessarily the model also validates
+  x + 1 -> l + 1 as:
+
+    min_premise m (l ∨ x + 1) = (min m[l] m[x]-1)+1 <= m[l] <-> m[x] <= m[l]
+
+  So, instead of checking d
+
+
+*)
+
+Class In T E := in_pred : E -> T -> Prop.
+Instance Ines : In LevelExprSet.t LevelExpr.t := LevelExprSet.In.
+Instance Inprems : In NES.t LevelExpr.t := fun x s => LevelExprSet.In x s.
+
+Notation " x ∈ S " := (in_pred x S) (at level 20).
+
+Equations remove_prem_opt (le : LevelExpr.t) (e : NES.t) : option NES.t :=
+  remove_prem_opt le e with inspect (LevelExprSet.is_empty (LevelExprSet.remove le e)) :=
+    | exist true _ => None
+    | exist false he => Some {| t_set := LevelExprSet.remove le e; t_ne := he |}.
+
+Lemma remove_prem_opt_Some le e e' le' :
+  remove_prem_opt le e = Some e' ->
+  LevelExprSet.In le' e' <->
+  LevelExprSet.In le' e /\ le <> le'.
+Proof.
+  funelim (remove_prem_opt le e) => //.
+  intros [= <-]; cbn.
+  rewrite LevelExprSet.remove_spec /LevelExprSet.E.eq.
+  intuition auto.
+Qed.
+
+Lemma remove_prem_opt_Some_eq le e e' :
+  le ∈ e ->
+  remove_prem_opt le e = Some e' ->
+  e = union (singleton le) e' /\ ~ le ∈ e'.
+Proof.
+  intros hin.
+  move/remove_prem_opt_Some => hl.
+  split.
+  - apply equal_exprsets => lk.
+    rewrite LevelExprSet.union_spec LevelExprSet.singleton_spec.
+    rewrite hl.
+    destruct (Classes.eq_dec lk le).
+    * subst. split => // _. now left.
+    * split => //. intros hin'. now right.
+      intros []. congruence. apply H.
+  - intros hin'. specialize (hl le).
+    apply hl in hin'. destruct hin'. congruence.
+Qed.
+
+Lemma remove_prem_opt_None le e :
+  remove_prem_opt le e = None ->
+  LevelExprSet.In le e <-> e = singleton le.
+Proof.
+  funelim (remove_prem_opt le e) => //.
+  intros _. clear H. move: e0.
+  rewrite LevelExprSet.is_empty_spec.
+  intros he.
+  split. intros.
+  - red in he.
+    apply equal_exprsets => l.
+    rewrite LevelExprSet.singleton_spec /LevelExprSet.E.eq.
+    split. intros hin.
+    setoid_rewrite LevelExprSet.remove_spec in he.
+    destruct (Classes.eq_dec l le0) => //.
+    elim (he l). split => //.
+    now intros ->.
+  - intros ->. now eapply LevelExprSet.singleton_spec.
+Qed.
+
+Definition union_opt (e : NES.t) (e' : option NES.t) : NES.t :=
+  match e' with
+  | Some e' => union e e'
+  | None => e
+  end.
+
+Lemma union_opt_union e e' e'' : union (union_opt e e') e'' = union e (union_opt e'' e').
+Proof.
+  destruct e'; cbn.
+  now rewrite union_assoc (@union_comm t0).
+  reflexivity.
+Qed.
+
+Lemma union_remove le prems :
+  le ∈ prems ->
+  union_opt (singleton le) (remove_prem_opt le prems) = prems.
+Proof.
+  intros hin.
+  destruct (remove_prem_opt le prems) eqn:hr.
+  - apply equal_exprsets => lk.
+    cbn. rsets; rewrite /LevelExprSet.E.eq.
+    eapply remove_prem_opt_Some in hr. erewrite hr.
+    firstorder auto. subst. apply hin.
+    destruct (Classes.eq_dec lk le). now left.
+    right. firstorder.
+  - apply remove_prem_opt_None in hr.
+    apply hr in hin. subst prems. now cbn.
+Qed.
+
+Lemma entails_weak_union_opt cls prems prems' concl :
+  entails cls (prems, concl) ->
+  entails cls (union_opt prems prems', concl).
+Proof.
+  destruct prems'; cbn => //.
+  now intros ent; rewrite union_comm; eapply entails_weak_union.
+Qed.
+
+Inductive max_chain cls : Clause.t -> Prop :=
+| incl cl : entails cls cl -> max_chain cls cl
+| chain {prems concl k k'} {prems' : NES.t} {concl'} :
+  max_chain cls (prems, (concl, k)) ->
+  max_chain cls (prems', concl') ->
+  (concl, k') ∈ prems' ->
+  max_chain cls (union_opt (add_prems (k' - k) prems) (remove_prem_opt (concl, k') prems'), concl').
+
+Lemma max_chain_entails cls cl :
+  max_chain cls cl <-> entails cls cl.
+Proof.
+  split.
+  + induction 1.
+    - exact H.
+    - eapply (entails_cumul_one (prems' := singleton (concl0, k'))); revgoals.
+      { rewrite union_opt_union union_remove //. now eapply entails_weak_union. }
+      eapply (entails_shift (k' - k)) in IHmax_chain1.
+      cbn in IHmax_chain1.
+      have heq: k' - k + k = k' by lia.
+      rewrite heq in IHmax_chain1.
+      eapply entails_all_singleton.
+      now eapply entails_weak_union_opt.
+  + intros ent; now apply incl.
+Qed.
+
+Definition thin_clause m cl :=
+  let prems := premise cl in
+  let filter '(l, k) := if entails_dec m (prems, (l, k + 1)) then false else true in
+  LevelExprSet.filter filter (premise cl).
+
+Lemma empty_filter f les :
+  LevelExprSet.is_empty (LevelExprSet.filter f les) ->
+  forall l, LevelExprSet.In l les -> f l = false.
+Proof.
+  move/LevelExprSet.is_empty_spec.
+  have hs := LevelExprSet.partition_spec2 (f:=f) les. forward hs. tc.
+  have hs' := LevelExprSet.partition_spec1 (f:=f) les. forward hs'. tc.
+  rewrite -hs'.
+  intros he l.
+  specialize (hs' l). specialize (hs l).
+  destruct (f l) eqn:hl.
+  rewrite LevelExprSet.filter_spec in hs'.
+  specialize (he l). rewrite hs' in he. intros hin; elim he; split => //.
+  auto.
+Qed.
+
+Lemma partition_in f les :
+  forall lk, LevelExprSet.In lk les <->
+    LevelExprSet.In lk (LevelExprSet.partition f les).1 \/
+    LevelExprSet.In lk (LevelExprSet.partition f les).2.
+Proof.
+  intros lk.
+  rewrite LevelExprSet.partition_spec1 LevelExprSet.partition_spec2.
+  rewrite !LevelExprSet.filter_spec.
+  firstorder auto.
+  destruct (f lk); firstorder.
+Qed.
+
+Lemma thin_clause_spec m cl :
+  let prems := thin_clause m cl in
+  if LevelExprSet.is_empty prems then
+    entails_all (clauses m) (premise cl) (succ (premise cl))
+  else
+    exists premsnl premsl,
+    [/\ premise cl = (union_opt premsnl premsl)%nes,
+      prems = premsnl,
+      (forall l k, (l, k) ∈ premsnl -> ~ entails (clauses m) (premise cl, (l, k+1))) &
+      on_Some_or_None (fun premsl => entails_all (clauses m) (premise cl) (succ premsl)) premsl].
+Proof.
+  intros prems.
+  destruct (LevelExprSet.is_empty prems) eqn:ise.
+  - have ha : forall l k, LevelExprSet.In (l, k) (premise cl) -> entails (clauses m) (premise cl, (l, k + 1)).
+    intros l k hin.
+    eapply (empty_filter _ _ ise) in hin.
+    destruct entails_dec => //.
+    move=> -[] l k /In_add_prems -[[l' k']] [] hin ->.
+    eapply ha in hin. rewrite /succ_expr //=. now rewrite Z.add_comm.
+  - subst prems; unfold thin_clause in *.
+    set (fn := fun '(l, k) => _) in *.
+    set (fil := LevelExprSet.filter _ _) in *.
+    have hs := LevelExprSet.partition_spec2 (f:=fn) (premise cl). forward hs. tc.
+    have hs' := LevelExprSet.partition_spec1 (f:=fn) (premise cl). forward hs'. tc.
+    set (part := LevelExprSet.partition _ _) in *.
+    exists {| t_set := fil; t_ne := ise |}.
+    destruct (LevelExprSet.is_empty part.2) eqn:ise2.
+    * exists None.
+      cbn. split => //.
+      { apply equal_exprsets; cbn.
+        move=> lk. rewrite LevelExprSet.filter_spec.
+        intuition auto.
+        rewrite hs in ise2.
+        have he := empty_filter _ _ ise2.
+        specialize (he lk H).
+        destruct (fn lk) => //. }
+      { move=> l k /LevelExprSet.filter_spec -[] hin hf hent.
+        unfold fn in hf. destruct entails_dec => //. }
+    * exists (Some {| t_set := part.2; t_ne := ise2 |}).
+      cbn. split => //.
+      apply equal_exprsets => l. cbn.
+      rewrite LevelExprSet.union_spec.
+      rewrite -[fil]hs'.
+      now rewrite -partition_in.
+      { move=> l k /LevelExprSet.filter_spec -[] hin' hf hent.
+        unfold fn in hf. destruct entails_dec => //. }
+      { move=> l /In_add_prems -[[le' le'k]] [].
+        cbn. rewrite hs => /LevelExprSet.filter_spec [] hin heq.
+        intros ->. unfold fn in heq. destruct entails_dec => //.
+        cbn in heq. now rewrite Z.add_comm. }
+Qed.
+
+Equations thin_clause_opt (m : t) (cl : clause) : option clause :=
+  | m, cl with inspect (LevelExprSet.is_empty (thin_clause m cl)) :=
+    | exist true _ => None
+    | exist false ne => Some ({| t_set := thin_clause m cl; t_ne := ne |}, concl cl).
+
+
+Lemma thin_clause_opt_spec m cl :
+  match thin_clause_opt m cl with
+  | None => False
+  | Some cl' =>
+    exists premsnl premsl,
+    [/\ premise cl = union_opt premsnl premsl,
+      cl' = (premsnl, concl cl),
+      (forall l k, (l, k) ∈ premsnl -> ~ entails (clauses m) (premise cl, (l, k+1))) &
+      on_Some_or_None (fun premsl => entails_all (clauses m) (premise cl) (succ premsl)) premsl]
+  end.
+Proof.
+  funelim (thin_clause_opt m cl); clear H.
+  - assert (h := thin_clause_spec m cl).
+    cbn in h.
+    rewrite e in h.
+    now eapply model_entails_loop in h.
+  - assert (h := thin_clause_spec m cl).
+    cbn in h.
+    clear Heqcall.
+    rewrite ne in h.
+    destruct h as [premsnl [premsl []]].
+    exists premsnl, premsl; split => //.
+    f_equal. apply equal_exprsets; cbn. now rewrite H0.
+Qed.
+
+Lemma interp_nes_thin_clause (v : Level.t -> Z) {m cl ne} {premsnl : NES.t} :
+  thin_clause m cl = premsnl ->
+  interp_nes v ({| t_set := thin_clause m cl; t_ne := ne |}) =
+  interp_nes v premsnl.
+Proof.
+  intros eq.
+  destruct premsnl.
+  destruct cl as [prems concl]; cbn in eq.
+  subst t_set0. f_equal.
+  apply equal_exprsets. cbn. reflexivity.
+Qed.
+
+Lemma interp_nes_union_opt v e e' :
+  interp_nes v (union_opt e e') =
+  match e' with
+  | Some e' => Z.max (interp_nes v e) (interp_nes v e')
+  | None => interp_nes v e
+  end.
+Proof.
+  destruct e' => //=.
+  now rewrite interp_nes_union; cbn.
+Qed.
+
+Lemma thin_clause_opt_valid m cl :
+  match thin_clause_opt m cl with
+  | None => False
+  | Some cl' => valid_clause_Z (clauses m) cl <-> valid_clause_Z (clauses m) cl'
+  end.
+Proof.
+  (* intros hent. *)
+  funelim (thin_clause_opt m cl).
+  - clear H Heqcall.
+    have hs := thin_clause_spec m cl.
+    cbn in hs. rewrite e in hs.
+    now eapply model_entails_loop in hs.
+  - clear H Heqcall.
+    have hs := thin_clause_spec m cl.
+    cbn in hs. rewrite ne in hs.
+    destruct cl as [prems [concl k]].
+    rewrite /valid_clause_Z. cbn.
+    cbn in hs. destruct hs as [premsl [premsnl [heq heq' hent' hentl]]].
+    split.
+    * move=> hv v vpos csem.
+      have hi := interp_nes_thin_clause v (ne := ne) heq'.
+      move: hv => /(_ v vpos csem).
+      rewrite hi. subst prems.
+      rewrite interp_nes_union_opt.
+      destruct premsnl => //.
+      destruct heq'.
+      move/to_entails_all: hentl.
+      move/entails_L_entails_ℋ_equiv/entails_L_rels_entails_L_clauses/completeness_all.
+      move/(_ Z _ v).
+      rewrite -interp_rels_clauses_sem.
+      move/(_ csem).
+      rewrite -interp_rels_clauses_sem.
+      move/clauses_sem_clauses_of_le.
+      rewrite interp_add_prems interp_nes_union.
+      cbn in hent' |- *. lia.
+    * move=> hv v vpos csem.
+      have hi := interp_nes_thin_clause v (ne := ne) heq'.
+      move: hv => /(_ v vpos csem).
+      rewrite hi.
+      subst prems.
+      rewrite interp_nes_union_opt.
+      destruct premsnl => //.
+      destruct heq'.
+      move/to_entails_all: hentl.
+      move/entails_L_entails_ℋ_equiv/entails_L_rels_entails_L_clauses/completeness_all.
+      move/(_ Z _ v).
+      rewrite -interp_rels_clauses_sem.
+      move/(_ csem).
+      rewrite -interp_rels_clauses_sem.
+      move/clauses_sem_clauses_of_le.
+      rewrite interp_add_prems interp_nes_union.
+      cbn in hent' |- *. lia.
+Qed.
+
+(*
+Lemma thin_clause_opt_entails m cl :
+  match thin_clause_opt m cl with
+  | None => False
+  | Some cl' => entails (clauses m) cl' -> entails (clauses m) cl
+  end.
+Proof. Admitted. *)
+
+Definition thin_clauses m :=
+  Clauses.fold (fun cl acc =>
+    match thin_clause_opt m cl with
+    | Some cl' => Clauses.add cl' acc
+    | None => acc (* Impossible for consistent models *)
+    end) (clauses m) Clauses.empty.
+
+Lemma thin_clauses_spec m :
+  forall cl, Clauses.In cl (clauses m) ->
+    exists cl', thin_clause_opt m cl = Some cl' /\ Clauses.In cl' (thin_clauses m).
+Proof. Admitted.
+
+Lemma thin_clauses_spec_inv m :
+  forall cl, Clauses.In cl (thin_clauses m) ->
+    exists clo, thin_clause_opt m clo = Some cl /\ Clauses.In clo (clauses m).
+Proof. Admitted.
+
+(** The thinned clauses are stronger than the original clauses *)
+Lemma thin_clauses_entails m : thin_clauses m ⊢ℋ clauses m.
+Proof.
+  intros cl hin.
+  destruct (thin_clauses_spec m cl hin) as [cl' [heq hin']].
+  have hs := thin_clause_opt_spec m cl.
+  rewrite heq in hs. destruct hs as [premsnl [premsl [eq eq' ent ent']]].
+  destruct cl as [prems concl]. cbn in eq, eq', ent.
+  subst prems cl'.
+  now eapply entails_weak_union_opt, entails_in.
+Qed.
+
+Lemma is_model_entails_H m cls cls' :
+  is_model m cls ->
+  cls ⊢ℋ cls' ->
+  is_model m cls'.
+Proof.
+  move=> /[dup] ism. rewrite !is_modelP.
+  move=> ha hent cl /hent ent.
+  specialize (ha cl).
+  eapply entails_model_valid; tea.
+Qed.
+
+Lemma thin_clauses_model model m :
+  is_model model (thin_clauses m) -> is_model model (clauses m).
+Proof.
+  move=> ism. eapply is_model_entails_H; tea.
+  eapply thin_clauses_entails.
+Qed.
+
+Lemma is_model_singleton m cl : is_model m (Clauses.singleton cl) <-> valid_clause m cl.
+Proof.
+  rewrite is_modelP. split.
+  * move/(_ cl) => /fwd //. clsets.
+  * now move=> hv cl' /Clauses.singleton_spec ->.
+Qed.
+
+Definition valid_non_vacuous m cl :=
+  exists minp value,
+    [/\ min_premise m (premise cl) = Some minp,
+       level_value m (concl cl).1 = Some value &
+       minp + (concl cl).2 <= value].
+
+Definition is_total_model_alt m cls :=
+  forall cl, Clauses.In cl cls -> valid_non_vacuous m cl.
+
+Lemma is_total_model_altP m cls :
+  is_total_model m cls <-> is_total_model_alt m cls.
+Proof.
+  split.
+  - move=> -[] en /is_modelP ism.
+    move=> [prems [concl k]] /[dup] /en [minp hmin] /ism.
+    move/valid_clause_elim/(_ _ hmin).
+    move/Some_leq => -[] z' [] hl hleq.
+    exists minp, z'. split => //.
+  - move=> ism; split.
+    * now move=> cl /ism -[] minp [] value [] => //; exists minp.
+    * apply/is_modelP => cl /ism -[] minp [] value [] => // hmin hl hle.
+      destruct cl as [prems [concl k]].
+      apply valid_clause_intro => z hz.
+      rewrite hmin in hz. noconf hz.
+      rewrite hl; constructor. exact hle.
+Qed.
+
+Lemma min_premise_union m prems prems' :
+  min_premise m (prems ∨ prems') = min_opt (min_premise m prems) (min_premise m prems').
+Proof.
+  pattern prems, (min_premise m prems).
+  set (P := fun t0 => _).
+  revert prems.
+  apply: (@min_premise_elim m _ _ _); subst P; cbn.
+  - intros le. now rewrite union_comm union_add_singleton min_premise_add.
+  - intros prems acc le he hnin.
+    rewrite -union_add_singleton (@union_comm prems) union_assoc union_comm union_add_singleton.
+    rewrite min_premise_add he.
+    now rewrite assoc.
+Qed.
+
+Lemma valid_clauses_of_le m prems prems' :
+  m ⊨ prems ⋞ prems' ->
+  forall min min', min_premise m prems' = Some min ->
+    min_premise m prems = Some min' ->
+    min <= min'.
+Proof.
+  revert prems'.
+  eapply min_premise_elim.
+  - intros [l k] prems'.
+    intros hl. specialize (hl (prems', (l, k))).
+    forward hl. rewrite clauses_of_le_spec. exists (l, k). split => //.
+    now apply singleton_spec. cbn in hl.
+    move/valid_clause_elim: hl => hz.
+    move=> min min' /hz /Some_leq -[y'] [] /level_value_MapsTo' hl leq hat.
+    rewrite (Model.min_atom_value_mapsto hl) in hat. cbn in hat. noconf hat. lia.
+  - intros prems' acc le ih hnin prems0 hadd min min' minp minp'.
+    move: (ih prems0) => /fwd.
+    { move=> cl. rewrite clauses_of_le_spec => -[lk [hin heq]].
+      move: (hadd cl) => /fwd //. subst cl. rewrite clauses_of_le_spec.
+      exists lk. split => //. eapply LevelExprSet.add_spec; now right. }
+    move=>/(_ _ _ minp).
+    destruct (min_atom_value m le) eqn:hat => //. destruct acc; noconf minp'.
+    2:{ cbn in minp'. destruct acc => //. }
+    move/(_ _ eq_refl).
+    move: (hadd (prems0, le)) => /fwd.
+    { rewrite clauses_of_le_spec. exists le. split => //.
+      eapply LevelExprSet.add_spec; now left. }
+    destruct le as [le lek]; move/valid_clause_elim/(_ _ minp) => /Some_leq.
+    apply min_atom_value_mapsto in hat. rewrite (level_value_MapsTo hat).
+    move=> -[y'] [] [=] <-. lia.
+Qed.
+
+Lemma is_total_model_thin m m' :
+  is_total_model m' (clauses m) ->
+  is_total_model m' (thin_clauses m).
+Proof.
+  move/is_total_model_altP => ism.
+  apply/is_total_model_altP => cl /thin_clauses_spec_inv -[] cl' [] heq /ism.
+  have := thin_clause_opt_spec m cl'.
+  rewrite heq => -[premsnl] [premsl] [eq eq' ent nent].
+  subst cl.
+  move=> -[] minp [] value [] => hmin hl hle.
+  exists minp, value. cbn. split => //.
+  rewrite -hmin eq.
+  apply antisymmetry; revgoals.
+  { eapply min_premise_subset. destruct premsl; cbn; lesets. }
+  destruct premsl as [premsl|]; cbn => //; revgoals. reflexivity.
+  rewrite min_premise_union.
+  cbn in nent.
+  rewrite -to_entails_all in nent.
+  eapply entails_all_model_valid in nent. 2:{ apply is_model_valid. eapply is_total_model_altP in ism. apply ism. }
+  rewrite eq in nent. cbn in nent.
+  rewrite eq min_premise_union in hmin.
+  destruct (min_premise m' premsl) as [minl|] eqn:minle, (min_premise m' premsnl) as [minnl|] eqn:minnle; cbn in hmin |- * => //.
+  noconf hmin. constructor.
+  eapply valid_clauses_of_le in nent. 2:{ rewrite min_premise_union minle minnle //=. }
+  2:{ rewrite (min_premise_add_prems minle); trea. } lia.
 Qed.
 
 Lemma check_clause_valid_Z m cl :
