common/theories/LoopChecking/ZModels.v
@@ -1,0 +1,315 @@
+
+
+Definition split_clauses m cls :=
+  Clauses.partition (is_enabled_clause m) cls.
+
+Definition enabled_clauses_of m cls := (split_clauses m cls).1.
+Definition disabled_clauses_of m cls := (split_clauses m cls).2.
+
+Lemma split_clauses_spec_1 m cls :
+  cls =_clset Clauses.union (enabled_clauses_of m cls) (disabled_clauses_of m cls).
+Proof. Admitted.
+
+Lemma enabled_clauses_spec m cl cls : Clauses.In cl (enabled_clauses_of m cls) <-> Clauses.In cl cls /\ enabled_clause m cl.
+Admitted.
+
+Lemma disabled_clauses_spec m cl cls : Clauses.In cl (disabled_clauses_of m cls) <-> Clauses.In cl cls /\ ~ enabled_clause m cl.
+Admitted.
+
+Lemma nenabled_clause m cl : ~ enabled_clause m cl <-> min_premise m (premise cl) = None.
+Proof.
+  case: (reflect_enabled m cl) => //.
+  split => //. red in p. firstorder. congruence.
+  firstorder. cbn in H. destruct min_premise => //.
+  destruct (H _ eq_refl).
+Qed.
+
+Lemma is_model_split m cls :
+  is_model m cls <-> (is_total_model m (enabled_clauses_of m cls)).
+Proof.
+  split.
+  - move/Clauses.for_all_spec => ism.
+    split.
+    intros cl. now rewrite enabled_clauses_spec. tc.
+    apply Clauses.for_all_spec. tc.
+    move=> cl /enabled_clauses_spec => -[] /ism //.
+  - move=> -[]. intros en. red in en. red in en.
+    intros ism. rewrite (split_clauses_spec_1 m cls).
+    eapply is_model_union. auto.
+    eapply Clauses.for_all_spec. tc.
+    move=> [prems [concl k]] /disabled_clauses_spec -[] hin hen.
+    Search enabled_clause.
+    apply valid_clause_intro.
+    now move/nenabled_clause: hen => ->.
+Qed.
+
+Lemma enabled_clause_defined {m cl} :
+  enabled_clause m cl ->
+  defined_model_of (NES.levels (premise cl)) m.
+Proof.
+  destruct cl as [prems [concl k]]; cbn.
+  move=> -[] z //= /min_premise_spec' hl.
+  move=> l /NES.levels_spec -[] k' /hl [v] [] hm _.
+  eapply level_value_MapsTo' in hm. now eexists.
+Qed.
+
+Lemma check_clause_invalid_Z cls cl mcheck :
+  check_gen cls cl = Invalid mcheck -> ~ valid_clause_Z (enabled_clauses_of mcheck cls) cl.
+Proof.
+  move/check_invalid => -[ism mof min en inv] nv.
+  destruct cl as [prems [concl k]].
+  destruct (level_value mcheck concl) eqn:he.
+  * specialize (nv (Z_valuation_of_model mcheck)).
+    forward nv. apply valuation_of_model_pos.
+    forward nv. apply is_model_split in ism.
+    apply valid_clauses_model. apply ism. apply ism.
+    move: nv.
+    rewrite def_clause_sem_valid.
+    unfold defined_model_of.
+    intros l; rewrite clause_levels_spec //=.
+    intros [hin|eq].
+    move/enabled_clause_defined: en.
+    now move/(_ _ hin). subst.
+    eapply level_value_MapsTo' in he. now eexists.
+    contradiction.
+  * apply is_model_split in ism.
+    destruct en as [minp eqmin].
+    remember (interp_nes (Z_valuation_of_model mcheck) prems) as iprems eqn:hprems.
+    symmetry in hprems.
+    set val := fun l =>
+      if l == concl then iprems + 1 - k
+      else Z_valuation_of_model mcheck l.
+    specialize (nv val).
+    forward nv. admit.
+    forward nv. admit.
+    move: nv; cbn.
+    rewrite {1}/val eqb_refl.
+    have eqi : interp_nes val prems = interp_nes (Z_valuation_of_model mcheck) prems.
+    move/min_premise_spec': eqmin => //=.
+    eapply interp_nes_elim. tc.
+    intros [le lek] h. rewrite /interp_expr.
+    rewrite interp_nes_singleton /interp_expr //=.
+    specialize (h le lek). admit.
+    intros. admit.
+    rewrite !eqi hprems. lia.
+Admitted.
+
+Lemma contra A B : (A -> B) -> (~ B -> ~ A).
+Proof. intros f nb a. exact (nb (f a)). Qed.
+
+Lemma invalid_clause_Z_ex cls cl :
+  (exists v : Level.t -> Z, positive_valuation v /\ clauses_sem v cls /\ ~ clause_sem v cl) ->
+   ~ valid_clause_Z cls cl.
+Proof.
+  intros [v [vpos [cs ncsem]]].
+  red. move/(_ v vpos cs). contradiction.
+Qed.
+
+(*
+  Check for validity in Z: cls |= cl.
+
+  Take an existing total model m of cls.
+  Add clauses low: v -> Set forall v. Ensure m[Set] = model_max m.
+  Add clauses high Set + 1 + (model_max - m[v]) -> v for every v, trivially
+  satisfied: as min_premise m [Set + 1 + (model_max m - m[v])] =
+    model_max m - (1 + (model_max m - model_min m)) = - 1 - model_min m <= m[v].
+
+  So m is also a total model of cls + low + high.
+  Launch checking for cls' ⊃ cls.
+  If we find a loop we get cls' |- loop, but as m is a total model of cls', that implies false in Z.
+  Otherwise we get a valid model [mcheck |= cls']
+  and either valid_clause mcheck cl or ~ valid_clause mcheck cl.
+  - If valid_clause mcheck cl, then
+    mcheck |= cls as cls ⊂ cls'.
+    So we have a valid clause in Zinf and Z, but not a proof
+    for every valuation...
+
+  E.g check x >= 0, y >= 0 -> x >= y.
+  adds 0 >= x and 0 >= y, forcing x = y = 0!
+  Add instead just 0 >= y, not better, it entails x >= y = 0.
+  Add instead just ⊥ + 1 >= y: starting from { x = 0; y = None; ⊥ = None }.
+  we get
+  { x = 0; y = None; ⊥ = 0 },
+  { x = 0; y = -1; ⊥ = 0 }. Good, does not entail x >= y
+  But x + 1 >= y ?
+  { x = 1; y = None; ⊥ = None } ->
+  { x = 1; y = None; ⊥ = 1 } ->
+  { x = 1; y = 0; ⊥ = 1 }.
+  Ok as well.
+
+  - If ~ valid_clause mcheck cl.
+    Then we have clauses_sem (Z_valuation_of_model mcheck) cls',
+    so clauses_sem (Z_valuation_of_model mcheck) cls, and
+    ~ clause_sem (Z_valuation_of_model mcheck) cl.
+*)
+
+Definition bound_clauses (m : Model.model) :=
+  LevelMap.fold (fun l k =>
+    Clauses.add (singleton (Level.zero, model_max m + 1 - option_get 0 k), (l, 0))) m Clauses.empty.
+
+Lemma bound_clauses_spec {cl m} :
+  Clauses.In cl (bound_clauses m) ->
+  exists l k, LevelMap.MapsTo l k m /\ cl = (singleton (Level.zero, model_max m + 1 - option_get 0 k), (l, 0)).
+Proof.
+  rewrite /bound_clauses.
+  set (mmax := model_max m). clearbody mmax.
+  eapply LevelMapFact.fold_rec.
+  - intros s' he hin. clsets.
+  - intros x a cls s' s'' hin hnin hadd ih.
+    rsets. destruct H.
+    * subst cl. exists x, a. split.
+      eapply levelmap_add_spec in hadd. rewrite hadd.
+      apply LevelMapFact.F.add_mapsto_iff. now left. reflexivity.
+    * eapply levelmap_add_spec in hadd.
+      specialize (ih H) as [l []]. exists l, x0. split => //.
+      rewrite hadd.
+      apply LevelMapFact.F.add_mapsto_iff. right; split => //.
+      intros ->. destruct H0. subst cl.
+      apply hnin; now eexists.
+      apply H0. apply H0.
+Qed.
+(*
+Lemma bound_clauses_spec_inv {l k V} :
+  LevelSet.In l V ->
+  Clauses.In (singleton (Level.zero, k), (l, 0)) (bound_clauses k V).
+Proof.
+  rewrite /bound_clauses.
+  eapply LevelSetProp.fold_rec.
+  - intros s' he hin. lsets.
+  - intros x a s' s'' hin hnin hadd ih.
+    rsets. apply hadd in H as [H|H].
+    * subst l. now left.
+    * specialize (ih H). now right.
+Qed. *)
+
+Lemma bound_clauses_prop m cls :
+  is_model m cls -> is_model m (bound_clauses m).
+Proof.
+  intros ism.
+  apply is_modelP => cl /bound_clauses_spec -[] l [k] [] hm heq.
+  subst cl.
+  apply valid_clause_intro => z.
+  rewrite min_premise_singleton /min_atom_value.
+  destruct level_value eqn:hl => //=.
+  have hz : z0 = model_max m. todo "zero spec".
+  subst z0.
+  intros [=].
+  have hzeq : z = - 1 + option_get 0 k. lia.
+  rewrite hzeq.
+  rewrite (level_value_MapsTo hm). destruct k. cbn in *; subst.
+  constructor. lia.
+  cbn in *. subst z.
+  todo "defined level".
+Qed.
+
+Lemma bound_clauses_ext m m' :
+  m' ⩽ m -> is_model m (bound_clauses m) -> is_model m' (bound_clauses m).
+Proof.
+  intros hext.
+Abort.
+
+
+Definition check_gen_Z (m : t) cl :=
+  check_gen (Clauses.union (bound_clauses m) (clauses m)) cl.
+
+Lemma enabled_clause_mcheck_zero_enabled mcheck cl cls :
+  enabled_clause mcheck cl ->
+  is_model mcheck cls ->
+  Deciders.above_zero_declared (clauses_levels cls) cls ->
+  exists k, LevelMap.MapsTo Level.zero (Some k) mcheck.
+Proof.
+Admitted.
+
+Lemma enabled_clause_mcheck_all_enabled mcheck cl cls :
+  enabled_clause mcheck cl ->
+  is_model mcheck cls ->
+  Deciders.above_zero_declared (clauses_levels cls) cls ->
+  forall l, LevelMap.In l mcheck -> exists k, LevelMap.MapsTo l (Some k) mcheck.
+Proof.
+Admitted.
+
+Lemma option_map_add_zero k : option_map (Z.add 0) k = k.
+Proof. destruct k => //. Qed.
+
+Lemma check_clause_invalid_Z_dis m cl :
+  clause_levels cl ⊂_lset levels m ->
+  check_gen_Z m cl = Valid -> valid_clause_Z (clauses m) cl.
+Proof.
+  intros hwf.
+  unfold check_gen_Z.
+  set (bcls := bound_clauses _).
+  set (cls' := Clauses.union _ _).
+  move/check_gen_entails.
+  rewrite entails_completeness.
+  intros hm. eapply valid_total_models_Z_models.
+  intros m' tot def.
+  specialize (hm (option Z) _ (opt_valuation_of_model m')).
+  apply clause_sem_valid. apply hm.
+  eapply clauses_sem_union.
+  destruct tot as [en ism].
+  split; revgoals.
+  eapply clauses_sem_valid; exact ism. revgoals. eauto.
+  have hmin : minimal_above (clauses m) (check_init_model (clauses m) cl) m.
+  admit.
+  red in hmin.
+  specialize (hmin m'). forward hmin. admit.
+  forward hmin. exact ism.
+  intros cl' hin.
+  eapply bound_clauses_spec in hin as [l [k [hm' heq]]].
+  subst cl'. cbn -[Semilattice.eq]. rewrite interp_nes_singleton /interp_expr.
+  rewrite /opt_valuation_of_model.
+  case: (find_spec l m').
+  intros k0 hml. destruct k0 => //. 2:{ todo "m' must have a value for l". }
+  case: (find_spec Level.zero m').
+  intros kz hmz. destruct kz. 2:{ todo "zero must have a value". }
+  rewrite option_map_add_zero.
+  destruct k.
+  have hmax : z0 = model_max m'. admit.
+  subst z0.
+  have hv := valuation_of_value_pos hml.
+  cbn -[Semilattice.le]. cbn.
+  eapply hmin in hm' as [k' []].
+  eapply LevelMapFact.F.MapsTo_fun in hml; tea. subst k'. depelim H0.
+  rewrite /valuation_of_value.
+  have hmleq : model_max m <= model_max m'. admit.
+  unfold valuation_of_value in hv.
+  have hv' := valuation_of_value_pos H0.
+  unfold valuation_of_value in hv'.
+  have hmeq : (model_max m' - model_max m' - model_min m') = - model_min m'. lia.
+  rewrite hmeq. lia.
+  cbn.
+  todo "scope".
+  todo "zero defined".
+  todo "zero defined".
+Qed.
+
+Lemma check_clause_invalid_Z_dis m cl mcheck :
+  clause_levels cl ⊂_lset levels m ->
+  check_gen_Z m cl = Invalid mcheck -> ~ valid_clause_Z (clauses m) cl.
+Proof.
+  intros hwf.
+  unfold check_gen_Z.
+  set (bcls := bound_clauses _ _).
+  set (cls' := Clauses.union _ _).
+  move/check_invalid => -[ism mof hmin en inval].
+  apply invalid_clause_Z_ex.
+  exists (Z_valuation_of_model mcheck).
+  split. apply valuation_of_model_pos.
+  have hab := above_zero_declared m.
+  have hdef0 : defined_model_of (clauses_levels cls') mcheck.
+  { eapply enabled_clause_defined in en.
+    specialize (hab (choose (premise cl)).1).
+    forward hab. apply hwf.
+    eapply clause_levels_spec. left.
+    eapply NES.levels_spec. exists (choose (premise cl)).2.
+    destruct (choose _) eqn:hc. cbn. rewrite -hc.
+    eapply choose_spec.
+    red in hab.
+  }
+  split.
+  eapply valid_clauses_model. admit.
+  eapply is_model_subset; tea. subst cls'; clsets.
+  intros csem.
+  eapply def_clause_sem_valid in csem. contradiction.
+  eapply enabled_clause_defined in en. admit.
+Qed.
